coq/proof/SimulationValid.v
@@ -16,10 +16,12 @@ Import Opsem.
 
 Require Import TODO.
 Require Import Decs.
+Require Import Hints.
 Require Import Validator.
 Require Import GenericValues.
 Require Import SimulationLocal.
 Require Import Simulation.
+Require Import Inject.
 Require InvMem.
 Require InvState.
 Require Import SoundBase.
@@ -32,64 +34,7 @@ Set Implicit Arguments.
 
 
 (* TODO: position *)
-Definition get_blocks (f:fdef): blocks :=
-  let '(fdef_intro _ blocks) := f in
-  blocks.
-
-Inductive vali_state_sim
-          (conf_src conf_tgt:Config)
-          (stack0_src stack0_tgt:ECStack)
-          (invmem:InvMem.Rel.t)
-          (idx:nat)
-          (st_src st_tgt:State): Prop :=
-| vali_state_sim_intro
-    m_src m_tgt
-    fdef_hint cmds_hint
-    inv inv_term
-    invst
-    (CONF: CONF_TODO) (* m_src, m_tgt, conf_src, conf_tgt *)
-    (ECS_SRC: st_src.(ECS) = stack0_src)
-    (ECS_TGT: st_tgt.(ECS) = stack0_tgt)
-    (FDEF: valid_fdef m_src m_tgt st_src.(EC).(CurFunction) st_tgt.(EC).(CurFunction) fdef_hint)
-    (CMDS: valid_cmds m_src m_tgt st_src.(EC).(CurCmds) st_tgt.(EC).(CurCmds) cmds_hint inv = Some inv_term)
-    (TERM: valid_terminator fdef_hint inv_term m_src m_tgt
-                            st_src.(EC).(CurFunction).(get_blocks)
-                            st_tgt.(EC).(CurFunction).(get_blocks)
-                            st_src.(EC).(CurBB).(fst)
-                            st_src.(EC).(Terminator)
-                            st_tgt.(EC).(Terminator))
-    (STATE: InvState.Rel.sem conf_src conf_tgt st_src st_tgt invst invmem inv)
-    (MEM: InvMem.Rel.sem conf_src conf_tgt st_src.(Mem) st_tgt.(Mem) invmem)
-.
-
-Lemma vali_init
-      m_src m_tgt
-      conf_src conf_tgt
-      stack0_src stack0_tgt
-      fdef_src fdef_tgt
-      fdef_hint
-      args_src args_tgt
-      mem_src mem_tgt
-      inv
-      ec_src
-      (FDEF: valid_fdef m_src m_tgt fdef_src fdef_tgt fdef_hint)
-      (ARGS: list_forall2 (genericvalues_inject.gv_inject inv.(InvMem.Rel.inject)) args_src args_tgt)
-      (MEM: InvMem.Rel.sem conf_src conf_tgt mem_src mem_tgt inv)
-      (CONF: CONF_TODO)
-      (INIT: init_fdef conf_src fdef_src args_src ec_src):
-  exists ec_tgt idx,
-    init_fdef conf_tgt fdef_tgt args_tgt ec_tgt /\
-    vali_state_sim
-      conf_src conf_tgt
-      stack0_src stack0_tgt
-      inv idx
-      (mkState ec_src stack0_src mem_src)
-      (mkState ec_tgt stack0_tgt mem_tgt).
-Proof.
-Admitted.
-
-(* TODO: position *)
-Ltac condtac :=
+Ltac simtac :=
   repeat
     (try match goal with
          | [H: ?a = ?a |- _] => clear H
@@ -133,39 +78,110 @@ Ltac condtac :=
      unfold Debug.debug_print_validation_process in *;
      try subst; ss).
 
-
 (* TODO: position *)
-Lemma inject_value_sound
-      conf_src st_src val_src
-      conf_tgt st_tgt val_tgt
-      invst invmem inv
-      gval_src
-      (STATE: InvState.Rel.sem conf_src conf_tgt st_src st_tgt invst invmem inv)
-      (MEM: InvMem.Rel.sem conf_src conf_tgt st_src.(Mem) st_tgt.(Mem) invmem)
-      (INJECT: Hints.Invariant.inject_value inv val_src val_tgt)
-      (VAL_SRC: InvState.Unary.sem_valueT conf_src st_src invst.(InvState.Rel.src) val_src = Some gval_src):
-  exists gval_tgt,
-    <<VAL_TGT: InvState.Unary.sem_valueT conf_tgt st_tgt invst.(InvState.Rel.tgt) val_tgt = Some gval_tgt>> /\
-    <<INJECT: genericvalues_inject.gv_inject invmem.(InvMem.Rel.inject) gval_src gval_tgt>>.
+Definition get_blocks (f:fdef): blocks :=
+  let '(fdef_intro _ blocks) := f in
+  blocks.
+
+Inductive valid_state_sim
+          (conf_src conf_tgt:Config)
+          (stack0_src stack0_tgt:ECStack)
+          (invmem:InvMem.Rel.t)
+          (idx:nat)
+          (st_src st_tgt:State): Prop :=
+| valid_state_sim_intro
+    m_src m_tgt
+    fdef_hint cmds_hint
+    inv inv_term
+    invst
+    (CONF: valid_conf m_src m_tgt conf_src conf_tgt)
+    (ECS_SRC: st_src.(ECS) = stack0_src)
+    (ECS_TGT: st_tgt.(ECS) = stack0_tgt)
+    (FDEF: valid_fdef m_src m_tgt st_src.(EC).(CurFunction) st_tgt.(EC).(CurFunction) fdef_hint)
+    (CMDS: valid_cmds m_src m_tgt st_src.(EC).(CurCmds) st_tgt.(EC).(CurCmds) cmds_hint inv = Some inv_term)
+    (TERM: valid_terminator fdef_hint inv_term m_src m_tgt
+                            st_src.(EC).(CurFunction).(get_blocks)
+                            st_tgt.(EC).(CurFunction).(get_blocks)
+                            st_src.(EC).(CurBB).(fst)
+                            st_src.(EC).(Terminator)
+                            st_tgt.(EC).(Terminator))
+    (STATE: InvState.Rel.sem conf_src conf_tgt st_src st_tgt invst invmem inv)
+    (MEM: InvMem.Rel.sem conf_src conf_tgt st_src.(Mem) st_tgt.(Mem) invmem)
+.
+
+Lemma valid_init
+      m_src m_tgt
+      conf_src conf_tgt
+      stack0_src stack0_tgt
+      fdef_src fdef_tgt
+      fdef_hint
+      args_src args_tgt
+      mem_src mem_tgt
+      inv idx
+      ec_src
+      (FDEF: valid_fdef m_src m_tgt fdef_src fdef_tgt fdef_hint)
+      (ARGS: list_forall2 (genericvalues_inject.gv_inject inv.(InvMem.Rel.inject)) args_src args_tgt)
+      (MEM: InvMem.Rel.sem conf_src conf_tgt mem_src mem_tgt inv)
+      (CONF: valid_conf m_src m_tgt conf_src conf_tgt)
+      (INIT_SRC: init_fdef conf_src fdef_src args_src ec_src):
+  exists ec_tgt,
+    <<INIT_TGT: init_fdef conf_tgt fdef_tgt args_tgt ec_tgt>> /\
+    <<SIM:
+      valid_state_sim
+        conf_src conf_tgt
+        stack0_src stack0_tgt
+        inv idx
+        (mkState ec_src stack0_src mem_src)
+        (mkState ec_tgt stack0_tgt mem_tgt)>>.
 Proof.
-Admitted.
+  inv INIT_SRC. unfold valid_fdef in FDEF. simtac.
+  exploit locals_init; eauto; [by apply CONF|]. i. des.
+  generalize FDEF. i.
+  unfold forallb2AL in FDEF0. ss. apply andb_true_iff in FDEF0. des. simtac.
+  hexploit InvState.Rel.sem_empty; eauto.
+  { instantiate (2 := mkEC _ _ _ _ _ _).
+    instantiate (1 := mkEC _ _ _ _ _ _).
+    s. eauto.
+  }
+  i. des.
+  esplits.
+  - econs; eauto. ss.
+  - econs; eauto. ss.
+    repeat
+      (try match goal with
+           | [|- is_true (if ?c then _ else _)] =>
+             let COND := fresh "COND" in
+             destruct c eqn:COND
+           end;
+       simtac).
+    { match goal with
+      | [H: proj_sumbool (fheader_dec ?a ?a) = false |- _] => destruct (fheader_dec a a); ss
+      end.
+    }
+    apply andb_true_iff. splits; [|by eauto].
+    repeat
+      (try match goal with
+           | [|- (if ?c then _ else _) = true] =>
+             let COND := fresh "COND" in
+             destruct c eqn:COND
+           end;
+       simtac).
+    { match goal with
+      | [H: proj_sumbool (id_dec ?a ?a) = false |- _] => destruct (id_dec a a); ss
+      end.
+    }
+    rewrite COND0, COND1, COND2, COND3, COND4. ss.
+Qed.
 
-(* TODO: position *)
-Lemma sem_valueT_physical
-      conf st inv val:
-  InvState.Unary.sem_valueT conf st inv (Exprs.ValueT.lift Exprs.Tag.physical val) =
-  getOperandValue conf.(CurTargetData) val st.(EC).(Locals) conf.(Globals).
-Proof. destruct val; ss. Qed.
-
-Lemma vali_sim
+Lemma valid_sim
       conf_src conf_tgt:
-  (vali_state_sim conf_src conf_tgt) <6= (sim_local conf_src conf_tgt).
+  (valid_state_sim conf_src conf_tgt) <6= (sim_local conf_src conf_tgt).
 Proof.
   intros stack0_src stack0_tgt.
   pcofix CIH.
   intros inv0 idx0 st_src st_tgt SIM. pfold.
   generalize (classic (stuck_state conf_src st_src)). intro STUCK_SRC. des.
-  { destruct (s_isFinialState conf_src st_src) eqn:FINAL_SRc; cycle 1.
+  { destruct (s_isFinialState conf_src st_src) eqn:FINAL_SRC; cycle 1.
     - (* error *)
       eapply _sim_local_error; eauto. econs; eauto.
     - (* final *)
@@ -173,27 +189,27 @@ Proof.
   }
   destruct st_src, st_tgt. destruct EC0, EC1.
   inv SIM. ss.
-  destruct CurCmds0; condtac;
+  destruct CurCmds0; simtac;
     (try by exfalso; eapply has_false_False; eauto).
   - (* term *)
     unfold valid_terminator in TERM.
-    condtac;
+    simtac;
       (try by exfalso; eapply has_false_False; eauto).
     apply NNPP in STUCK_SRC. des.
-    inv STUCK_SRC; destruct Terminator1; condtac.
+    inv STUCK_SRC; destruct Terminator1; simtac.
     (* TODO: switch case *)
     + (* return *)
-      unfold returnUpdateLocals in *. condtac.
-      exploit inject_value_sound; eauto.
-      { rewrite sem_valueT_physical. eauto. }
-      rewrite sem_valueT_physical. s. i. des.
+      unfold returnUpdateLocals in *. simtac.
+      exploit InvState.Rel.inject_value_spec; eauto.
+      { rewrite InvState.Unary.sem_valueT_physical. eauto. }
+      rewrite InvState.Unary.sem_valueT_physical. s. i. des.
       eapply _sim_local_return; eauto; ss.
     + (* return_void *)
       eapply _sim_local_return_void; eauto; ss.
     + (* br *)
-      exploit inject_value_sound; eauto.
-      { rewrite sem_valueT_physical. eauto. }
-      rewrite sem_valueT_physical. s. i. des.
+      exploit InvState.Rel.inject_value_spec; eauto.
+      { rewrite InvState.Unary.sem_valueT_physical. eauto. }
+      rewrite InvState.Unary.sem_valueT_physical. s. i. des.
       eapply _sim_local_step.
       { admit. (* tgt not stuck *) }
       i. inv STEP. ss.
@@ -240,19 +256,21 @@ Proof.
       * admit. (* valid_terminator *)
 Admitted.
 
-Lemma vali_sim_fdef
+Lemma valid_sim_fdef
       m_src m_tgt
       conf_src conf_tgt
       fdef_src fdef_tgt
       fdef_hint
-      (CONF: CONF_TODO)
+      (CONF: valid_conf m_src m_tgt conf_src conf_tgt)
       (FDEF: valid_fdef m_src m_tgt fdef_src fdef_tgt fdef_hint):
   sim_fdef conf_src conf_tgt fdef_src fdef_tgt.
 Proof.
   ii.
-  exploit vali_init; eauto. i. des.
+  exploit valid_init; eauto. i. des.
   esplits; eauto.
-  apply vali_sim; eauto.
+  apply valid_sim; eauto.
+Grab Existential Variables.
+  { exact 0%nat. }
 Qed.
 
 Lemma valid_products_lookupFdefViaIDFromProducts
@@ -269,20 +287,20 @@ Proof.
   induction products_src; [done|].
   i. destruct products_tgt; [done|].
   unfold valid_products in PRODUCTS. s in PRODUCTS. apply andb_true_iff in PRODUCTS. des.
-  s in SRC. condtac.
-  - destruct a, p; condtac. esplits; eauto.
+  s in SRC. simtac.
+  - destruct a, p; simtac. esplits; eauto.
     + destruct (getFdefID fdef0 == getFdefID fdef_src); eauto. congruence.
     + destruct (id_dec (getFdefID fdef_src) (getFdefID fdef0)); ss.
       destruct (valid_fdef m_src m_tgt fdef_src fdef0 f0) eqn:FDEF; ss. congruence.
-  - destruct a, p; condtac. congruence.
+  - destruct a, p; simtac. congruence.
   - exploit IHproducts_src; eauto. i. des.
     esplits; eauto.
     destruct (lookupFdefViaIDFromProduct p f) eqn:HD; ss.
-    destruct a, p; condtac.
+    destruct a, p; simtac.
   - exploit IHproducts_src; eauto. i. des.
     esplits; eauto.
     destruct (lookupFdefViaIDFromProduct p f) eqn:HD; ss.
-    destruct a, p; condtac.
+    destruct a, p; simtac.
 Qed.
 
 Lemma valid_products_genGlobalAndInitMem
@@ -302,7 +320,7 @@ Proof.
   revert products_tgt globals locals mem PRODUCTS.
   induction products_src; i; destruct products_tgt; ss.
   unfold valid_products in PRODUCTS. ss. apply andb_true_iff in PRODUCTS. des.
-  destruct a, p; condtac.
+  destruct a, p; simtac.
   - apply Decs.gvar_eqb_spec in COND. subst.
     destruct gvar0; ss.
     + destruct (initGlobal (layouts, namedts) globals mem0 id5 typ5 const5 align5) as [[]|]; eauto.
@@ -315,30 +333,33 @@ Proof.
     destruct (initFunTable mem0 id0); eauto.
 Qed.
 
-Lemma vali_sim_module m_hint:
+Lemma valid_sim_module m_hint:
   (valid_module m_hint) <2= sim_module.
 Proof.
   s. intros module_src module_tgt MODULE.
-  unfold valid_module in MODULE. condtac.
-  ii. unfold s_genInitState in SRC. condtac.
+  unfold valid_module in MODULE. simtac.
+  ii. unfold s_genInitState in SRC. simtac.
   clear COND0 e0. apply infrastructure_props.InProductsB_In in e.
-  exploit valid_products_lookupFdefViaIDFromProducts; eauto. i. des. condtac.
+  exploit valid_products_lookupFdefViaIDFromProducts; eauto. i. des. simtac.
   destruct fheader5. inv e0. ss.
   esplits.
   - unfold s_genInitState. ss. rewrite TGT.
     match goal with
     | [|- context [productInModuleB_dec ?a ?b]] => destruct (productInModuleB_dec a b)
-    end; condtac; cycle 1.
-    { eadmit. (* lookupFdefViaIDFromProducts -> InProductsB *) }
+    end; simtac; cycle 1.
+    { admit. (* lookupFdefViaIDFromProducts -> InProductsB *) }
     unfold initTargetData in *.
     erewrite <- valid_products_genGlobalAndInitMem; eauto. rewrite COND2.
     rewrite COND3. eauto.
   - apply sim_local_lift_sim. econs.
     + econs 1.
     + generalize H0. i.
-      unfold forallb2AL in H1. ss. apply andb_true_iff in H1. des. condtac.
-      apply vali_sim. econs; eauto.
-      * admit. (* CONF_TODO *)
+      unfold forallb2AL in H1. ss. apply andb_true_iff in H1. des. simtac.
+      hexploit InvState.Rel.sem_empty; eauto.
+      { admit. (* init_locals inject_locals *) }
+      i. des.
+      apply valid_sim. econs; eauto.
+      * admit. (* valid_conf *)
       * (* TODO: reorganize tactics *)
         repeat
           (try match goal with
@@ -346,7 +367,7 @@ Proof.
                  let COND := fresh "COND" in
                  destruct c eqn:COND
                end;
-           condtac).
+           simtac).
         { match goal with
           | [H: proj_sumbool (fheader_dec ?a ?a) = false |- _] => destruct (fheader_dec a a); ss
           end.
@@ -358,13 +379,12 @@ Proof.
                  let COND := fresh "COND" in
                  destruct c eqn:COND
                end;
-           condtac).
+           simtac).
         { match goal with
           | [H: proj_sumbool (id_dec ?a ?a) = false |- _] => destruct (id_dec a a); ss
           end.
         }
         rewrite COND5, COND6, COND7, COND8, COND9. ss.
-      * admit. (* state *)
-      * admit. (* mem *)
+      * ss. admit. (* InvMem.Rel.sem init_mem *)
     + reflexivity.
 Admitted.
