coq/proof/SoundBase.v
@@ -18,7 +18,14 @@ Require Import TODO.
 Require Import Validator.
 Require Import GenericValues.
 Require Import SimulationLocal.
+Require Import Inject.
 Require InvMem.
 Require InvState.
 
-Definition CONF_TODO: Prop. Admitted.
+(* TODO: m_src, m_tgt, conf_src, conf_tgt *)
+Inductive valid_conf
+          (m_src m_tgt:module)
+          (conf_src conf_tgt:Config): Prop :=
+| valid_conf_intro
+    (INJECT: inject_conf conf_src conf_tgt)
+.
