coq/proof/SoundImplies.v
@@ -26,10 +26,10 @@ Set Implicit Arguments.
 
 
 Lemma implies_sound
-      conf_src st_src
-      conf_tgt st_tgt
+      m_src conf_src st_src
+      m_tgt conf_tgt st_tgt
       invst invmem inv0 inv1
-      (CONF: CONF_TODO) (* m_src, m_tgt, conf_src, conf_tgt *)
+      (CONF: valid_conf m_src m_tgt conf_src conf_tgt)
       (IMPLIES: Hints.Invariant.implies inv0 inv1)
       (STATE: InvState.Rel.sem conf_src conf_tgt st_src st_tgt invst invmem inv0)
       (MEM: InvMem.Rel.sem conf_src conf_tgt st_src.(Mem) st_tgt.(Mem) invmem):
