coq/proof/SoundReduceMaydiff.v
@@ -26,10 +26,11 @@ Set Implicit Arguments.
 
 
 Lemma reduce_maydiff_sound
+      m_src m_tgt
       conf_src st_src
       conf_tgt st_tgt
       invst invmem inv
-      (CONF: CONF_TODO) (* m_src, m_tgt, conf_src, conf_tgt *)
+      (CONF: valid_conf m_src m_tgt conf_src conf_tgt)
       (STATE: InvState.Rel.sem conf_src conf_tgt st_src st_tgt invst invmem inv)
       (MEM: InvMem.Rel.sem conf_src conf_tgt st_src.(Mem) st_tgt.(Mem) invmem):
   <<STATE: InvState.Rel.sem conf_src conf_tgt st_src st_tgt invst invmem
